### Dot Product

$$
    ||\vec u - \vec v||^2 = ||\vec u||^2 + ||\vec v||^2 - 2||\vec u|| ||\vec v||\cos(\theta) \\
$$

$$
    \begin{align*}
        ||\vec u||^2 = u_1^2 + u_2^2 + u_3^2 \\
        ||\vec v||^2 = v_1^2 + v_2^2 + v_3^2 \\
    \end{align*}
$$

$$
    \begin{align*}
        ||\vec u - \vec v||^2 & = (u_1 - v_1)^2 + (u_2 - v_2)^2 + (u_3 - v_3)^2 \\ & = (u_1^2 - 2u_1v_1 + v_1^2) + (u_2^2 - 2u_2v_2 + v_2^2) + (u_3^2 - 2u_3v_3 + v_3^2) \\ & = (u_1^2 + u_2^2 + u_3^2) + (v_1^2 + v_2^2 + v_3^2) - 2(u_1v_1 + u_2v_2 + u_3v_3) 
    \end{align*}
$$

$$
    \begin{align*}
        \theta & = \cos^{-1}(\dfrac{u_1v_1 + u_2v_2 + u_3v_3}{||\vec u|| ||\vec v||}) \\ & = \cos^{-1}(\dfrac{\vec u \cdot \vec v}{||\vec u|| ||\vec v||})
    \end{align*}
$$

