名古屋大学　大学院情報学研究科　2012年度博士前期課程入試問題 工３

\[1] $F(s)$ = $\dfrac{4}{s^4+4}$ を逆ラプラス変換せよ。

$$
    \begin{align*}
        s^4 + 4 & = (s^4+4+4s^2) - 4s^2 = (s^2+2)^2 - 4s^2  \\\ 
        & = (s^2+2-2s)(s^2+2+2s) = (s^2+2s+2)(s^2-2s+2)
    \end{align*}
$$

$$
    \begin{align*}
          & \dfrac{4}{s^4+4} = \dfrac{As+B}{s^2+2s+2} + \dfrac{Cs+D}{s^2-2s+2} \\\
          & 4 = (As+B)(s^2-2s+2) + (Cs+D)(s^2+2s+2)
    \end{align*}
$$

$$
    \begin{align*}
         \begin{cases} 
            A + C = 0 \\\
            B + D = 2 \\\
            -2A + B + 2C + D = 0 \\\
            2A -2B + 2C + 2D = 0  
         \end{cases}
    \end{align*}
$$

$$
    \begin{pmatrix} 
        1 & 0 & 1 & 0 & 0 \\\
        1 & -1 & 1 & 1 & 0 \\\
        0 & 1 & 0 & 1 & 2 \\\
        -2 & 1 & 2 & 2 & 0 
    \end{pmatrix} \to 
    \begin{pmatrix} 
        1 & 0 & 1 & 0 & 0 \\\
        0 & 1 & 0 & -1 & 0 \\\
        0 & 0 & 2 & 1 & 0 \\\
        0 & 0 & 0 & 1 & 1 
    \end{pmatrix} 
$$

$$
    A = 1/2, \quad B = D = 1, \quad C = -1/2
$$

$$
    \begin{align*}
        f(t) & = \dfrac{1}{2}\mathscr{L^{-1}}[\dfrac{s+2}{s^2+2s+2} - \dfrac{s - 2}{s^2-2s+2}] \\\
        & = \dfrac{1}{2}\mathscr{L^{-1}}[\dfrac{s+1+1}{(s+1)^2 + 1^2}] - \dfrac{1}{2}\mathscr{L^{-1}}[\dfrac{s-1-1}{(s-1)^2 +1^2}] \\\
        & = \dfrac{1}{2}[e^{-t}(\cos(t)+\sin(t))] - \dfrac{1}{2}[e^{t}(\cos(t)-\sin(t))] \\\
        & = \dfrac{1}{2}[e^{-t}(\cos(t) + \sin(t)) -e^{t}(\cos(t)-\sin(t))]
    \end{align*}
$$